Saturation framework: proof that lexicographic extension of wf ordering is wf in progress

Saturation_Framework/Given_Clause.thy
@@ -45,9 +45,68 @@ definition equiv_F_fun :: "'f \<Rightarrow> 'f \<Rightarrow> bool" (infix "\<dot
 definition Prec_eq_F :: "'f \<Rightarrow> 'f \<Rightarrow> bool" (infix "\<lless>\<doteq>" 50) where
   "Prec_eq_F C D \<equiv> ((C,D) \<in> Equiv_F \<or> C \<lless> D)"
 
-definition Prec_Fl :: "('f \<times> 'l) \<Rightarrow> ('f \<times> 'l) \<Rightarrow> bool" (infix "\<sqsubset>" 50) where
-  "Prec_Fl Cl1 Cl2 \<equiv> (fst Cl1 \<lless> fst Cl2) \<or> (fst Cl1 \<doteq> fst Cl2 \<and> snd Cl1 \<sqsubset>l snd Cl2)"
+definition Prec_FL :: "('f \<times> 'l) \<Rightarrow> ('f \<times> 'l) \<Rightarrow> bool" (infix "\<sqsubset>" 50) where
+  "Prec_FL Cl1 Cl2 \<equiv> (fst Cl1 \<lless> fst Cl2) \<or> (fst Cl1 \<doteq> fst Cl2 \<and> snd Cl1 \<sqsubset>l snd Cl2)"
 
+find_theorems minimal_element
+
+lemma "minimal_element (\<sqsubset>) UNIV"
+proof
+  show "po_on (\<sqsubset>) UNIV" unfolding po_on_def
+  proof
+    show "irreflp_on (\<sqsubset>) UNIV" unfolding irreflp_on_def Prec_FL_def
+    proof
+      fix a
+      assume a_in: "a \<in> (UNIV::('f \<times> 'l) set)"
+      have "\<not> (fst a \<lless> fst a)" using wf_prec_F minimal_element.min_elt_ex by force
+      moreover have "\<not> (snd a \<sqsubset>l snd a)" using wf_prec_l minimal_element.min_elt_ex by force
+      ultimately show "\<not> (fst a \<lless> fst a \<or> fst a \<doteq> fst a \<and> snd a \<sqsubset>l snd a)" by blast
+    qed
+  next
+    show "transp_on (\<sqsubset>) UNIV" unfolding transp_on_def Prec_FL_def
+    proof (simp, intro allI impI)
+      fix a1 b1 a2 b2 a3 b3
+      assume trans_hyp:"(a1 \<lless> a2 \<or> a1 \<doteq> a2 \<and> b1 \<sqsubset>l b2) \<and> (a2 \<lless> a3 \<or> a2 \<doteq> a3 \<and> b2 \<sqsubset>l b3)"
+      have "a1 \<lless> a2 \<Longrightarrow> a2 \<lless> a3 \<Longrightarrow> a1 \<lless> a3" using wf_prec_F compat_equiv_prec by blast
+      moreover have "a1 \<lless> a2 \<Longrightarrow> a2 \<doteq> a3 \<Longrightarrow> a1 \<lless> a3" using wf_prec_F compat_equiv_prec by blast
+      moreover have "a1 \<doteq> a2 \<Longrightarrow> a2 \<lless> a3 \<Longrightarrow> a1 \<lless> a3" using wf_prec_F compat_equiv_prec by blast
+      moreover have "b1 \<sqsubset>l b2 \<Longrightarrow> b2 \<sqsubset>l b3 \<Longrightarrow> b1 \<sqsubset>l b3"
+        using wf_prec_l unfolding minimal_element_def po_on_def transp_on_def by (meson UNIV_I)
+      moreover have "a1 \<doteq> a2 \<Longrightarrow> a2 \<doteq> a3 \<Longrightarrow> a1 \<doteq> a3"
+        using equiv_F_is_equiv_rel equiv_class_eq unfolding equiv_F_fun_def by fastforce
+      ultimately show "(a1 \<lless> a3 \<or> a1 \<doteq> a3 \<and> b1 \<sqsubset>l b3)" using trans_hyp by blast
+    qed
+  qed
+next
+  show "wfp_on (\<sqsubset>) UNIV" unfolding wfp_on_def 
+  proof
+    assume contra: "\<exists>f. \<forall>i. f i \<in> UNIV \<and> f (Suc i) \<sqsubset> f i"
+    then obtain f where f_in: "\<forall>i. f i \<in> UNIV" and f_suc: "f (Suc i) \<sqsubset> f i" by blast
+    (* define f_F where "f_F i = *)
+oops
+
+lemma labeled_static_ref_comp:
+  "static_refutational_complete_calculus Bot_FL Inf_FL (\<Turnstile>\<inter>L) with_labels.Red_Inf_Q with_labels.Red_F_Q"
+  using labeled_static_ref[OF static_ref_comp] .
+
+lemma standard_labeled_lifting_family: "q \<in> Q \<Longrightarrow> lifting_with_wf_ordering_family Bot_FL Inf_FL Bot_G (entails_q q) Inf_G (Red_Inf_q q) (Red_F_q q) (\<G>_F_L_q q) (\<G>_Inf_L_q q) (\<lambda>g. Prec_FL)"
+proof -
+  fix q
+  assume q_in: "q \<in> Q"
+  have "lifting_with_wf_ordering_family Bot_FL Inf_FL Bot_G (entails_q q) Inf_G
+    (Red_Inf_q q) (Red_F_q q) (\<G>_F_L_q q) (\<G>_Inf_L_q q) (\<lambda>g. Labeled_Empty_Order)"
+    using ord_fam_lifted_q[OF q_in] .
+  then have "standard_lifting Bot_FL Inf_FL Bot_G Inf_G (entails_q q) (Red_Inf_q q) (Red_F_q q)
+    (\<G>_F_L_q q) (\<G>_Inf_L_q q)"
+    using lifted_q q_in by blast
+  moreover have "minimal_element Prec_FL UNIV"
+    unfolding Prec_FL_def using wf_prec_F wf_prec_l 
+  ultimately show "lifting_with_wf_ordering_family Bot_FL Inf_FL Bot_G (entails_q q) Inf_G (Red_Inf_q q) (Red_F_q q) (\<G>_F_L_q q) (\<G>_Inf_L_q q) (\<lambda>g. Prec_FL)" 
+oops
+
+sublocale lifting_equivalence_with_red_crit_family Inf_FL Bot_G Inf_G Q entails_q Red_Inf_q Red_F_q
+  Bot_FL \<G>_F_L_q \<G>_Inf_L_q "\<lambda>g. Prec_FL"
+  sorry
 
 end
 
